\noindent \textbf{Question 1}: Write the complete problem: kinematic + static + constitutive equation! \\

\textbf{Answer:} Kinematic admissibility:

\begin{equation}
\underline{u} \cdot \underline{n} = 0 \quad \forall \Mu \in S_{Lat} \rightarrow u_r = 0 \quad \forall \Mu \in S_{Lat} 
\end{equation}
\begin{equation}
\underline{n} \cdot \underline{u}  = -U \quad \forall \Mu \in S_{z}^+ \rightarrow u_z = -U \quad \forall \Mu \in S_{z}^+ 
\end{equation}
\begin{equation}
\epsuu (\underline{u}) = \frac{1}{2} ({\Graduu \uu + \Graduu^T \uu }) \quad \forall \Mu \in \Omega
\end{equation}
\begin{equation}
\underline{u} \cdot \underline{n} = 0 \quad \forall \Mu \in S_{z}^- \rightarrow u_z = 0 \quad \forall \Mu \in S_{z}^- 
\end{equation} \\

Static admissibility:
\begin{equation}
\divu \sigmauu = \underline{0} \quad \forall \Mu \in \Omega 
\end{equation}
or in expanded form as below
\begin{equation}
\begin{split}
& \sigmarr ,_r + \frac{1}{r} (\sigmart,_\theta + \sigmarr - \sigmatt) + \sigmarz,_z = 0 \\
& \sigmatr ,_r + \frac{1}{r} (\sigmatt,_\theta + \sigmart + \sigmatr) + \sigmatz,_z = 0 \\
& \sigmazr ,_r + \frac{1}{r} (\sigmazt,_\theta + \sigmazr ) + \sigmazz,_z = 0
\end{split} \quad \quad  \rightarrow \quad \quad \forall \Mu \in \Omega 
\end{equation}

Contact without friction:
\begin{equation}
(\sigmauu \cdot \tu)\cdot \tu = 0 \quad \forall \Mu \in S_z^+ \rightarrow \sigmarz = \sigmatz = 0 \quad \Mu \in S_z^+
\label{eq:szplus}
\end{equation}

Contact without friction:
\begin{equation}
(\sigmauu \cdot \tu)\cdot \tu = 0 \quad \forall \Mu \in S_z^- \rightarrow \sigmarz = \sigmatz = 0 \quad \Mu \in S_z^-
\label{eq:szmin}
\end{equation}

Contact without friction:
\begin{equation}
(\sigmauu \cdot \tu)\cdot \tu = 0 \quad \forall \Mu \in S_{Lat} \rightarrow \sigmatr = \sigmatz = 0 \quad \Mu \in S_{Lat}
\label{eq:slat}
\end{equation}

Constitutive equations:
\begin{equation}
\sigmauu = \lambda \text{tr} \epsuu \underline{\underline{1}} + 2 \mu \epsuu \quad \forall \Mu \in \Omega
\end{equation}



\noindent \textbf{Question 2}: Assume that $\uu = - \frac{U}{h} z \eu_z $. Is this kinematically admissible? \\

\textbf{Answer:} We assume that
\begin{equation}
\uu = \left(
\begin{matrix}
0 \\ 0 \\ -\frac{U}{h}z
\end{matrix}
\right) = \left(
-\frac{U}{h}z
\right) \quad \text{Of course } \uu \text{ is kinematically admissible.}
\end{equation}
By definition (using the gradient of a vector with cylindrical coordinates):
\begin{equation}
\Graduu \cdot \uu = \left[
\begin{matrix}
0 &0 &0 \\
0 &0 &0 \\
0 &0 &-\frac{U}{h} \\
\end{matrix}
\right] \rightarrow \epsuu = \left[
\begin{matrix}
0 &0 &0 \\
0 &0 &0 \\
0 &0 & \epszz \\
\end{matrix}
\right]
\end{equation}
with $\epszz = -U/h \rightarrow $ the compatibility equation is obviously satisfied. \\

\noindent \textbf{Question 3}: Find the corresponding stress $\sigmauu$. Is it statistically admissible? \\

\textbf{Answer:} 
\begin{equation}
\sigmauu = \lambda \text{tr} \epsuu \underline{\underline{1}} + 2 \mu \epsuu \rightarrow \sigmauu = \left[
\begin{matrix}
-\lambda \frac{U}{h} &0 &0 \\
0 &-\lambda \frac{U}{h} &0 \\
0 &0 & -(\lambda+2\mu) \frac{U}{h} \\
\end{matrix}
\right]
\end{equation} 
Eqs. \ref{eq:slat}, \ref{eq:szmin}, and \ref{eq:szplus} are obviously satisfied.
$\divu \sigmauu \rightarrow$ obviously equal to 0 as $\sigmauu $ is constant. \\

\noindent \textbf{Question 4}: Find oedometric  modulus $\hat{E}$ as a  function of $E$ and $\nu$.

\textbf{Answer:} The vertical force is equal to 
\begin{equation}
\Pu = \int_{S_z^+} \sigmauu \cdot \eu_z dS_3^+
\end{equation}
\begin{equation}
\Pu = \int_{S_z^+} - (\lambda + 2\mu)\frac{U}{h} dS_3^+ \eu_z = -\Pu \eu_z \quad \text{with} \quad \Pu = \frac{(\lambda+2\mu)US}{h} 
\end{equation}
So we can identify the oedometric modulus $\hat{E} = \lambda + 2\mu$.

\begin{equation}
\begin{split}
 \sigmauu &= \lambda \text{tr} \epsuu \underline{\underline{1}} + 2 \mu \epsuu \\
 \epsuu &= \frac{1+\nu}{E} \sigmauu - \frac{\nu}{E} \text{tr} \sigmauu \underline{\underline{1}}
\end{split} \quad \rightarrow \quad  
\begin{split}
\text{tr} \sigmauu &= (3\lambda + 2\mu) \text{  tr} \epsuu \\
\text{tr} \epsuu &= (\frac{1-2\nu}{E}) \text{  tr} \sigmauu \\
\end{split} \quad \rightarrow \quad 3\lambda + 2\mu = \frac{E}{1-2\nu}
\end{equation}

Or we can also write as follows:
\begin{equation}
\text{tr} \sigmauu = (3\lambda + 2\mu) \text{tr} \epsuu \quad \rightarrow \quad \sigmauu = \frac{\lambda}{3\lambda + 2\mu} \text{tr} \sigmauu \underline{\underline{1}} + 2\mu \epsuu
\end{equation}
\begin{equation}
\epsuu = \frac{1}{2\mu} \sigmauu - \frac{\lambda}{2\mu (3\lambda + 2\mu)} \text{tr} \sigmauu \underline{\underline{1}}
\end{equation}

By identification, 
\begin{equation}
\frac{1}{2\mu} = \frac{1+\nu}{E} \quad  \text{     and     } \quad \frac{\lambda}{2\mu (3\lambda + 2\mu)} = \frac{\nu}{E}  
\end{equation}
\begin{equation}
\rightarrow \lambda = \frac{E \nu}{(1+\nu)(1-2\nu)} \quad  \text{     and     } \quad \mu = \frac{E}{2(1+\nu)}
\end{equation}
Thus, 
\begin{equation}
\hat{E} = \lambda + 2\mu = \frac{2 E\nu + 2E(1-2\nu)}{2(1+\nu)(1-2\nu)} = \frac{E(1-\nu)}{(1+\nu)(1-2\nu)}
\end{equation}
